very nice

Cm/PiE/Ast.lean
@@ -124,7 +124,7 @@ inductive Expr where
   -- for forming cons types
   | unit   : Expr
   | prod   : Level → Level → Expr
-  | nil    : Expr -- nil : Unit
+  | nil    : Level → Expr -- nil {α : Type} : α → Unit
   -- the core combinators: π, const, apply, id, eq, both
   -- these have explicit universe level arguments
   | apply  : Level → Level → Expr
@@ -157,14 +157,18 @@ notation "f$" => Expr.app
 notation "×'" => Expr.prod
 notation "Ty" => Expr.ty
 
-abbrev mk_quote (m n : Level) (α β x : Expr) : Expr := ::[::[const' m n, α, β], x]
-
 inductive Error where
   | stuck      : Expr → Error
   | no_rule    : Expr → Error
 deriving BEq, DecidableEq
 
 open Expr
+
+def Expr.push (l with_val : Expr) : Expr :=
+  match l with
+  | :: x xs => :: x (Expr.push xs with_val)
+  | nil m => :: with_val (nil m)
+  | x => :: x with_val
 
 /-
 Foldls cons'd pairs / lists
@@ -191,7 +195,7 @@ partial def Expr.fmt (e : Expr) : Format :=
   | const' m n => "const'.{" ++ [m, n].toString ++ "}"
   | both m n o => "both.{" ++ [m, n, o].toString ++ "}"
   | both' m n o => "both'.{" ++ [m, n, o].toString ++ "}"
-  | nil => "nil"
+  | nil m => "nil.{" ++ [m].toString ++ "}"
   | prod m n => "×'.{" ++ [m, n].toString ++ "}"
   | unit => "Unit"
   | Ty n => s!"Ty {n}"
