Cm/PiE/Eval.lean
@@ -12,41 +12,39 @@ This mirrors is_step_once exactly.
 -/
 def do_step_apply : Expr → Except Error Expr
   -- this apply rule allows treating a list as if it were a function application
-  | ::[::[.id _o, _α], x] => pure x
-  | e@::[::[(const _o _p), _α, _β], _c]
-  | e@::[::[(const' _o _p), _α, _β], _c] => pure e
-  | ::[::[::[(const _o _p), _α, _β], c], _x]
-  | ::[::[::[(const' _o _p), _α, _β], c], _x] => pure c
-  | ::[::[::[(both o p q), α, β, γ], ::[f, g]], x] =>
-    pure <| ::[f$ (apply o p) ::[::[α, β], ::[f, x]], f$ (apply o q) ::[::[α, γ], ::[g, x]]]
-  | ::[::[::[(both' o p q), α, β, γ], ::[f, g]], x] =>
+  | ::[.id _o, _α, x] => pure x
+  | ::[const _o _p, _α, _β, c, _x]
+  | ::[const' _o _p, _α, _β, c, _x] => pure c
+  | ::[both o p q, α, β, γ, ::[f, g], x] => -- TODO: not sure whether to nest ::[f, g] here, or leave flat
+    pure <| ::[f$ (apply o p) ::[α, β, f, x], f$ (apply o q) ::[α, γ, g, x]]
+  | ::[both' o p q, α, β, γ, ::[f, g], x] =>
     -- both' is nondependent, so β' = (mk_quote p.succ o (Ty p) α β)
     let fβ := mk_quote p.succ o (Ty p) α β
     let gβ := mk_quote q.succ o (Ty q) α γ
 
-    pure <| ::[f$ (apply o p.succ) ::[::[α, fβ], ::[f, x]], f$ (apply o q.succ) ::[::[α, gβ], ::[g, x]]]
-  | ::[::[::[π o p q r, α, β, γ, δ], ::[fx, fxs]], ::[x, xs]] =>
-    pure <| ::[f$ (apply o q) ::[::[α, γ], ::[fx, x]], f$ (apply p r) ::[::[β, δ], ::[fxs, xs]]]
-  | ::[::[::[::[eq _o _p, _α, _β], fn_yes, fn_no], a], b] =>
+    pure <| ::[f$ (apply o p.succ) ::[α, fβ, f, x], f$ (apply o q.succ) ::[α, gβ, g, x]]
+  | ::[π o p q r, α, β, γ, δ, ::[fx, fxs], ::[x, xs]] =>
+    pure <| ::[f$ (apply o q) ::[α, γ, fx, x], f$ (apply p r) ::[β, δ, fxs, xs]]
+  | ::[eq o p, α, β, ::[fn_yes, fn_no], a, b] =>
     if a == b then
-      pure <| f$ fn_yes a
+      pure <| f$ (apply o p) ::[α, β, fn_yes, a]
     else
-      pure <| f$ fn_no b
+      pure <| f$ (apply o p) ::[α, β, fn_no, b]
   | e => .error <| .no_rule e
 
 def run (e : Expr) : Except Error Expr := do
   match e with
-  | f$ a@(apply _m _n) ::[::[fα, fβ], ::[f, x]] => do
+  | f$ a@(apply _m _n) ::[fα, fβ, f, x] => do
     let eval_both : Except Error Expr := do
       let f' ← run f
       let x' ← run x
-      pure <| f$ a ::[::[fα, fβ], ::[f', x']]
+      pure <| f$ a ::[fα, fβ, f', x']
     let eval_arg_first : Except Error Expr := do
       let x' ← run x
-      pure <| f$ a ::[::[fα, fβ], ::[f, x']]
+      pure <| f$ a ::[fα, fβ, f, x']
     let eval_f_first : Except Error Expr := do
       let f' ← run f
-      pure <| f$ a ::[::[fα, fβ], ::[f', x]]
+      pure <| f$ a ::[fα, fβ, f', x]
     let step_whole : Except Error Expr := do
       do_step_apply <| ::[f, x]
 
@@ -71,6 +69,8 @@ def try_step_n (n : ℕ) (e : Expr) : Except Error Expr :=
 
 namespace hole
 
+def π? (fx 
+
 def quote (e : Expr) : Expr := ::[::[const' 0 0, ?, ?], e]
 def quote?₁ (α e : Expr) (m : Option Level := .none) : Expr := ::[::[const' (m.getD 0) 0, α, ?], e]
 
@@ -87,8 +87,8 @@ def both?₀ (α : Option Expr := .none) (m : Option Level := .none) : Expr :=
   , (α.getD .hole)
   , ? , ?]
 
-def apply?₀ (α β : Option Expr := .none) (m n : Option Level := .none) : Expr :=
-  f$ (f$ (apply (m.getD 0) (n.getD 0)) (α.getD ?)) (β.getD ?)
+def mkapp? (e : Expr) (α β : Option Expr := .none) (m n : Option Level := .none) : Expr :=
+  f$ (apply (m.getD 0) (n.getD 0)) ::[::[α.getD .hole, β.getD .hole], e]
 
 def id? (α : Option Expr := .none) (m : Option Level := .none) := ::[id (m.getD 0), α.getD .hole]
 
@@ -105,7 +105,7 @@ def both?_n (n : ℕ) (f g : Expr) (α : Option Expr := .none) (m : Option Level
   ((List.range n).tail.map (fun n => quote?_n n both?₀)).foldr
     (fun e acc => both? e acc) (both? (f := f) (g := g) (α := α) (m := m))
 
-example : try_step_n 200 (f$ apply?₀ ::[(f$ apply?₀ ::[(f$ apply?₀ ::[quote?_n 3 (Ty 0), (Ty 0)]), Ty 0]), Ty 0])  = (.ok (Ty 0)) := rfl
+example : try_step_n 200 (mkapp? ::[mkapp? ::[mkapp? ::[quote?_n 3 (Ty 0), (Ty 0)], Ty 0], Ty 0])  = (.ok (Ty 0)) := rfl
 
 /-
   α → β
@@ -131,21 +131,12 @@ def apply.type_with_holes.mk_β (m n : Level) : Expr :=
    (m := m.succ)
 
 -- (Ty 0) → (Ty 2)
-#eval try_step_n 200 (f$ apply?₀ ::[apply.type_with_holes.mk_β 1 2
+--#eval try_step_n 200 (mkapp? ::[apply.type_with_holes.mk_β 1 2
 
 /-
-apply : ∀ (α : Type) (β : α → Type) : ∀ (l : ((∀ (x : α), β x) × α)), l.fst l.snd
+id : ∀ (l : ((α : Type) × α)), l.fst
 
-apply : (:: both (:: (quote (Type m)) (:: both (:: (
--/
-def apply.type_with_holes (m : Level) : Expr :=
-  both?₁
-    (α := (Ty m))
-    (f := (quote?₁ (α := Ty 
-  sorry
-
-/-
-id : ∀ (α : Type), α → α
+id : :: π 
 -/
 def id.type_with_holes (m : Level) : Expr :=
   both?
@@ -160,17 +151,25 @@ def id.type_with_holes (m : Level) : Expr :=
         (m := m.succ)))
       (m := m.succ)))
 
-example : Expr.tail! <$> try_step_n 500 (f$ apply?₀ ::[id.type_with_holes 0, Ty 0])
-  >>= (fun (e : Expr) => try_step_n 500 (f$ apply?₀ ::[e, Ty 100])) = (.ok (::[Ty 0, Ty 0])) := rfl
+/-
+const' : ∀ (α : Type) (β : Type) (x : α) (y : β x), α
+
+-/
+def const'.type_with_holes (m n : Level) : Expr :=
+  sorry
+
+example : Expr.tail! <$> try_step_n 500 (mkapp? ::[id.type_with_holes 0, Ty 0])
+  >>= (fun (e : Expr) => try_step_n 500 (mkapp? ::[e, Ty 100])) = (.ok (::[Ty 0, Ty 0])) := rfl
 
 /-
 Type inference for filling in holes in expr types.
 -/
-def infer_holes : Expr → Except Error Expr
-  |
+/-def infer_holes : Expr → Except Error Expr
+  |-/
+
+example : try_step_n 100 (mkapp? ::[::[id 2, Ty 1], Ty 0]) = (.ok <| Ty 0) := rfl
+
+example : try_step_n 100 (mkapp? ::[::[::[const 2 2, Ty 1, Ty 1], Ty 0], Ty 0]) = (.ok <| Ty 0) := rfl
 
 end hole
 
-example : try_step_n 100 (f$ (f$ (f$ (apply 0 0) nil) nil) ::[::[id 2, Ty 1], Ty 0]) = (.ok <| Ty 0) := rfl
-
-example : try_step_n 100 (f$ (f$ (f$ (apply 0 0) nil) nil) ::[::[::[const 2 2, Ty 1, Ty 1], Ty 0], Ty 0]) = (.ok <| Ty 0) := rfl
